lean/example.lean
@@ -1,0 +1,25 @@
+
+import lean.language
+
+inductive lang : Type
+| skip            : lang
+| assign          : string → IncLoLang.expression → lang
+| non_det_assign  : string → lang
+| seq             : lang → lang → lang
+| if_             : IncLoLang.expression → lang → lang → lang
+| loop_           : IncLoLang.expression → lang → lang
+| error           : lang
+
+def lang.to_stmt : lang → IncLoLang.stmt 
+| lang.skip := IncLoLang.stmt.skip
+| (lang.assign s e) := IncLoLang.stmt.assign s e
+| (lang.non_det_assign s) := IncLoLang.stmt.non_det_assign s
+| (lang.seq C₁ C₂) := IncLoLang.stmt.seq (C₁.to_stmt) (C₂.to_stmt)
+| (lang.if_ e bt bf) := (IncLoLang.stmt.assumes (λ st, e st = 0) ;; (bt.to_stmt)) <+> (IncLoLang.stmt.assumes (λ st, e st ≠ 0) ;; (bf.to_stmt))
+| (lang.loop_ e l) := (IncLoLang.stmt.assumes (λ st, e st = 0) ;; (l.to_stmt))** ;; IncLoLang.stmt.assumes (λ st, e st ≠ 0)
+| lang.error := IncLoLang.stmt.error
+
+-- instance : has_repr IncLoLang.stmt :=
+--   λ x, "A"
+
+notation a `;>` b := lang.seq a b
